src/dafny/beacon/forkchoice/ForkChoiceProofs.p.dfy
@@ -23,6 +23,8 @@ include "ForkChoiceHelpers.dfy"
 include "../attestations/AttestationsTypes.dfy"
 include "../attestations/AttestationsHelpers.dfy"
 include "../Helpers.dfy"
+include "../BeaconChainTypes.dfy"
+include "../statetransition/EpochProcessing.s.dfy"
 
 /**
  *  Proofs for the ForkChoice properties.  
@@ -40,6 +42,8 @@ module ForckChoiceProofs {
     import opened AttestationsTypes
     import opened AttestationsHelpers
     import opened BeaconHelpers
+    import opened BeaconChainTypes
+    import opened EpochProcessingSpec
 
     /**
      *  RuleI for slashing. 
@@ -49,21 +53,6 @@ module ForckChoiceProofs {
     // {
     //     forall a1, a2 :: a1 in xa && a2 in xa ==>
 
-    // }
-
-    /**
-     *  
-     */
-    // function collectAttestationsForEpoch(xa: seq<PendingAttestation>, e : Epoch) : nat 
-    //     ensures collectAttestationsForEpoch(xa, e) <= |xa|
-    // {
-    //     if |xa| == 0 then 
-    //         0
-    //     else 
-    //         if compute_epoch_at_slot(xa[0].data.slot) == e then 
-    //             1 + collectAttestationsForEpoch(xa[1..], e)
-    //         else 
-    //             collectAttestationsForEpoch(xa[1..], e)                  
     // }
 
 
@@ -90,8 +79,8 @@ module ForckChoiceProofs {
                     var sl1 := store.blocks[roots1[0]].slot;  //  slot of br1 as a block
                     var sl2 := store.blocks[roots2[0]].slot;  //  slot of br2 as a block
                     //  compute the indices of EBBs in roots.
-                    var ebbsIndices1 := computeAllEBBs(roots1, compute_epoch_at_slot(sl1), store);
-                    var ebbsIndices2 := computeAllEBBs(roots2, compute_epoch_at_slot(sl2), store);
+                    var ebbsIndices1 := computeAllEBBsIndices(roots1, compute_epoch_at_slot(sl1), store);
+                    var ebbsIndices2 := computeAllEBBsIndices(roots2, compute_epoch_at_slot(sl2), store);
                     //  given 0 <= j < compute_epoch_at_slot(sl), (roots[j],j) is the EBB at
                     //  epoch(B) - j
                     true
@@ -121,18 +110,18 @@ module ForckChoiceProofs {
             var chbr1 := chainRoots(br1, store);
             var chbr2 := chainRoots(br2 , store);
             //  EBB(br1, j) is k1[0]
-            var k1 := computeAllEBBs(chbr1, j, store);
+            var k1 := computeAllEBBsIndices(chbr1, j, store);
             //  EBB(br1, j) is k1[0]
-            var k2 := computeAllEBBs(chbr2, j, store);
+            var k2 := computeAllEBBsIndices(chbr2, j, store);
             isJustified(0, chbr1, k1, links) && isJustified(0, chbr2, k2, links)
 
         ensures 
             var chbr1 := chainRoots(br1, store);
             var chbr2 := chainRoots(br2 , store);
             //  EBB(br1, j) is k1[0]
-            var k1 := computeAllEBBs(chbr1, j, store);
+            var k1 := computeAllEBBsIndices(chbr1, j, store);
             //  EBB(br1, j) is k1[0]
-            var k2 := computeAllEBBs(chbr2, j, store);
+            var k2 := computeAllEBBsIndices(chbr2, j, store);
             var tgt1 := CheckPoint(0 as Epoch, chbr1[k1[0]]);
             var tgt2 := CheckPoint(0 as Epoch, chbr2[k2[0]]);
             |collectAttestationsForTarget(links, tgt1) * collectAttestationsForTarget(links, tgt2)|
@@ -142,9 +131,9 @@ module ForckChoiceProofs {
         var chbr2 : seq<Root> := chainRoots(br2, store); //  chain(br2)
 
         //  compute the indices of EBBs in roots. Because j > 0, |k1| == j + 1 > 1.
-        var k1 := computeAllEBBs(chbr1, j, store);
+        var k1 := computeAllEBBsIndices(chbr1, j, store);
         //  EBB(br1, j) is k1[0]
-        var k2 := computeAllEBBs(chbr2, j, store);
+        var k2 := computeAllEBBsIndices(chbr2, j, store);
         //  EBB(br2, j) is k2[0]
 
         if (isJustified(0, chbr1, k1, links) && isJustified(0, chbr2, k2, links)) {
@@ -173,17 +162,6 @@ module ForckChoiceProofs {
         // assert(cp1 != cp2);
     }
 
-    lemma {:induction k} foo102(x : set<nat>, k : nat) 
-        requires x == set x: nat | 0 <= x < k :: x
-        ensures |x| == k
-    {
-        if k == 0 {
-            //  Thanks Dafny
-        } else {
-            foo102(x - {k - 1}, k - 1);
-        }
-    }
-
     /**
      *  If two aggregation bits have nore than 2/3 of  MAX_VALIDATORS_PER_COMMITTEE
      *  set to true, then the bitwise intersection of `xa` and `xb` has more than 
@@ -199,7 +177,7 @@ module ForckChoiceProofs {
         ensures |trueBitsCount(xa) * trueBitsCount(xb)| >= MAX_VALIDATORS_PER_COMMITTEE / 3 + 1
     {
         var k := set x: nat | 0 <= x < MAX_VALIDATORS_PER_COMMITTEE :: x;
-        foo102(k, MAX_VALIDATORS_PER_COMMITTEE);
+        successiveNatSetCardBound(k, MAX_VALIDATORS_PER_COMMITTEE);
         assert(|k| == MAX_VALIDATORS_PER_COMMITTEE);
         pigeonHolePrinciple(trueBitsCount(xa), trueBitsCount(xb), k);
     }
@@ -211,74 +189,9 @@ module ForckChoiceProofs {
         ensures |collectAttestationsForTarget(xa, tgt1) * collectAttestationsForTarget(xa, tgt2)| >= MAX_VALIDATORS_PER_COMMITTEE / 3 + 1
     {
         var k := set x: nat | 0 <= x < MAX_VALIDATORS_PER_COMMITTEE :: x;
-        foo102(k, MAX_VALIDATORS_PER_COMMITTEE);
+        successiveNatSetCardBound(k, MAX_VALIDATORS_PER_COMMITTEE);
         assert(|k| == MAX_VALIDATORS_PER_COMMITTEE);
         pigeonHolePrinciple(collectAttestationsForTarget(xa, tgt1), collectAttestationsForTarget(xa, tgt2), k);
     }
 
-    // lemma pigeonHolePrincipleForSeq(x: seq<int>, y : seq<int>, z : seq<int>) 
-    //     requires forall i, j :: 0 <= i < j < |z| ==> z[i] != z[j]
-    //     requires forall i, j :: 0 <= i < j < |x| ==> x[i] != x[j]
-    //     requires forall i, j :: 0 <= i < j < |y| ==> y[i] != y[j]
-    //     requires |x| >= 2 * |z| / 3 + 1   //    or equivalently 2 * |z| < 3 * |x| 
-    //     requires |y| >= 2 * |z| / 3 + 1   //    or equivalently 2 * |z| < 3 * |y|
-    //     ensures |x * y| >= |z| / 3 + 1    //    or equivalently 3 * |x * y| < |z| 
-
-    // {
-    //     pigeonHolePrinciple(x, y, z);   
-    // }
-
-   /**
-    *  If two finite sets x and y are included in another one z and
-    *  have more than 2/3(|z|) elements, then their intersection has more
-    *  then |z|/3 elements.
-    */
-    lemma pigeonHolePrinciple(x: set<int>, y : set<int>, z : set<int>)
-        requires  x <= z 
-        requires y <= z
-        requires |x| >= 2 * |z| / 3 + 1   //    or equivalently 2 * |z| < 3 * |x| 
-        requires |y| >= 2 * |z| / 3 + 1   //    or equivalently 2 * |z| < 3 * |y|
-        ensures |x * y| >= |z| / 3 + 1    //    or equivalently 3 * |x * y| < |z| 
-    {
-        //  Proof of alternative assumption
-        // assert(|x| >= 2 * |z| / 3 + 1 <==> 2 * |z| < 3 * |x|);
-        // assert(|y| >= 2 * |z| / 3 + 1 <==> 2 * |z| < 3 * |y|);
-        //  Proof by contradiction
-        if |x * y| < |z| / 3 + 1 {
-            //  size of union is sum of sizes minus size of intersection.
-            calc == {
-                |x + y|;
-                |x| + |y| - |x * y|;
-            }
-            cardIsMonotonic(x + y, z);
-        } 
-        //  proof of alternative conclusion
-        // assert(3 * |x * y| > |z| <==> |x * y| >= |z| / 3 + 1 );
-    } 
-
-   /**
-    *  If a finite set x is included in a finite set y, then
-    *  card(x) <= card(y).
-    *
-    *  @param  T   A type.
-    *  @param  x   A finite set.
-    *  @param  y   A finite set.
-    *  @returns    A proof that x <= y implies card(x) <= card(y)
-    *              in other terms, card(_) is monotonic.
-    */
-    // lemma cardIsMonotonic<T>(x : set<T>, y : set<T>) 
-    //     requires x <= y 
-    //     ensures |x| <= |y|
-    //     decreases y 
-    // {
-    //     if |y| == 0 {
-    //         //  Thanks Dafny
-    //     } else {
-    //         //  |y| >= 1, get an element in y
-    //         var e :| e in y;
-    //         var y' := y - { e };
-    //         //  Split recursion according to whether e in x or not
-    //         cardIsMonotonic(if e in x then x - {e} else x, y');
-    //     }
-    // }
 }
