src/dafny/beacon/statetransition/EpochProcessing.p.dfy
@@ -1,0 +1,381 @@
+/*
+ * Copyright 2020 ConsenSys Software Inc.
+ *
+ * Licensed under the Apache License, Version 2.0 (the "License"); you may 
+ * not use this file except in compliance with the License. You may obtain 
+ * a copy of the License at http://www.apache.org/licenses/LICENSE-2.0
+ *
+ * Unless required by applicable law or agreed to in writing, software dis-
+ * tributed under the License is distributed on an "AS IS" BASIS, WITHOUT 
+ * WARRANTIES OR CONDITIONS OF ANY KIND, either express or implied. See the 
+ * License for the specific language governing permissions and limitations 
+ * under the License.
+ */
+
+include "../../utils/Eth2Types.dfy"
+include "../../utils/SetHelpers.dfy"
+include "../../ssz/Constants.dfy"
+include "../forkchoice/ForkChoiceTypes.dfy"
+include "../forkchoice/ForkChoiceHelpers.dfy"
+include "../attestations/AttestationsTypes.dfy"
+include "../attestations/AttestationsHelpers.dfy"
+include "../Helpers.dfy"
+include "../BeaconChainTypes.dfy"
+include "../statetransition/EpochProcessing.s.dfy"
+include "EpochProcessingHelpers.dfy"
+
+/**
+ *  Proofs for the ForkChoice properties.  
+ */
+module EpochProcessingProofs {
+    
+    //  Import some constants, types and beacon chain helpers.
+    import opened Eth2Types
+    import opened Constants
+    import opened ForkChoiceTypes
+    import opened ForkChoiceHelpers
+    import opened AttestationsTypes
+    import opened AttestationsHelpers
+    import opened BeaconHelpers
+    import opened BeaconChainTypes
+    import opened EpochProcessingSpec
+    import opened EpochProcessingHelpers
+
+    /**
+     *  RuleI for slashing. 
+     *  A validator cannot vote more than once for a given epoch.
+     */
+    // predicate ruleI(xa : seq<PendingAttestation>) 
+    // {
+    //     forall a1, a2 :: a1 in xa && a2 in xa ==>
+
+    // }
+    /**
+     *  The last justified checkpoint in view(s).
+     */
+
+    // function lastJustifiedCheckPoint(s: BeaconState, store: Store) : CheckPoint 
+    //     requires get_current_epoch(s) as nat *  SLOTS_PER_EPOCH as nat  <  0x10000000000000000 
+    //     requires get_current_epoch(s) *  SLOTS_PER_EPOCH   < s.slot  
+    //     requires s.slot  - get_current_epoch(s)  *  SLOTS_PER_EPOCH <= SLOTS_PER_HISTORICAL_ROOT 
+    //     requires get_block_root(s, get_current_epoch(s)) in store.blocks.Keys
+    //     requires isClosedUnderParent(store)
+    // {
+    //     var r := get_block_root(s, get_current_epoch(s));
+    //     var roots := chainRoots(r, store); 
+    //     //  |ebbsIndices| ==  get_current_epoch(s) + 1
+    //     var ebbsIndices := computeAllEBBsIndices(roots, get_current_epoch(s), store);
+    //     var lastJustified := lastJustified(roots, ebbsIndices, store.attestations);
+    //     CheckPoint((|ebbsIndices| - 1 - lastJustified) as Epoch, roots[ebbsIndices[lastJustified]])
+    // }
+
+
+    /**
+     *  Whether a checkpoint is justified in the view that corresponds to a state.
+     */
+    // predicate isJustifiedCheckPoint(cp : CheckPoint, s: BeaconState, store: Store) 
+    //     requires get_current_epoch(s) as nat *  SLOTS_PER_EPOCH as nat  <  0x10000000000000000 
+    //     requires get_current_epoch(s) *  SLOTS_PER_EPOCH   < s.slot  
+    //     requires s.slot  - get_current_epoch(s)  *  SLOTS_PER_EPOCH <= SLOTS_PER_HISTORICAL_ROOT 
+    //     requires get_block_root(s, get_current_epoch(s)) in store.blocks.Keys
+    //     requires isClosedUnderParent(store)
+
+    // {
+    //     var r := get_block_root(s, get_current_epoch(s));
+    //     var roots := chainRoots(r, store); 
+    //     var ebbsIndices := computeAllEBBsIndices(roots, get_current_epoch(s), store);
+    //     exists i :: 0 <= i < |ebbsIndices| && isJustified(i, roots, ebbsIndices, store.attestations)
+    //         && cp == CheckPoint((|ebbsIndices| - i) as Epoch, roots[ebbsIndices[i]])
+    // }
+
+    /**
+     *  If a checkpoint is justified and there is a supermajority link from it to 
+     *  a more recent one, the more recent one is justified too.
+     */
+    lemma addJustified(cp1 : CheckPoint, cp2: CheckPoint, s: BeaconState, store: Store, links: seq<PendingAttestation>) 
+        requires get_current_epoch(s) as nat *  SLOTS_PER_EPOCH as nat  <  0x10000000000000000 
+        requires get_current_epoch(s) *  SLOTS_PER_EPOCH   < s.slot  
+        requires s.slot  - get_current_epoch(s)  *  SLOTS_PER_EPOCH <= SLOTS_PER_HISTORICAL_ROOT 
+        requires get_block_root(s, get_current_epoch(s)) in store.blocks.Keys
+        requires isClosedUnderParent(store)
+
+        requires isJustifiedCheckPoint(cp1, s, store)
+        //  cp2 is a checkpoint in view(s)
+        // requires exists 
+        requires |collectAttestationsForLink(
+                    links, 
+                    cp1, 
+                    cp2)| 
+                        >= (2 * MAX_VALIDATORS_PER_COMMITTEE) / 3 + 1
+        // requires  
+    {
+
+    }
+
+
+    /**
+     *  Whether a checkpoint is the most recent justified in the view from s.
+     */
+    // predicate isMostRecentJustifiedCheckPoint(cp : CheckPoint, s: BeaconState, store: Store) 
+    //     requires get_current_epoch(s) as nat *  SLOTS_PER_EPOCH as nat  <  0x10000000000000000 
+    //     requires get_current_epoch(s) *  SLOTS_PER_EPOCH   < s.slot  
+    //     requires s.slot  - get_current_epoch(s)  *  SLOTS_PER_EPOCH <= SLOTS_PER_HISTORICAL_ROOT 
+    //     requires get_block_root(s, get_current_epoch(s)) in store.blocks.Keys
+    //     requires isClosedUnderParent(store)
+
+    // {
+    //     var r := get_block_root(s, get_current_epoch(s));
+    //     var roots := chainRoots(r, store); 
+    //     var ebbsIndices := computeAllEBBsIndices(roots, get_current_epoch(s), store);
+    //     // exists i :: 0 <= i < |ebbsIndices| && isJustified(i, roots, ebbsIndices, store.
+    //     var lastJustified := lastJustified(roots, ebbsIndices, store.attestations);
+    //     cp == CheckPoint((|ebbsIndices| - lastJustified) as Epoch, roots[ebbsIndices[lastJustified]])
+    // }
+
+    /**
+     *  Given a state `s`, and the attestations in s.current_epoch_attestations,
+     *  if they are all valid they must originate from LJ(s).
+     *
+     *  @param  s       A state.
+     *  @param  store   A store with all the received attestations.
+     *  
+     *  @note           This lemma is not trivial and assumed for now.
+     */
+    lemma validAttestationsHaveSourceLJ(s : BeaconState, store:  Store)
+        requires s.slot % SLOTS_PER_EPOCH != 0
+        requires get_current_epoch(s) as nat *  SLOTS_PER_EPOCH as nat  <  0x10000000000000000 
+        requires get_current_epoch(s) > GENESIS_EPOCH + 1
+        requires get_current_epoch(s) *  SLOTS_PER_EPOCH   < s.slot  
+        requires s.slot  - get_current_epoch(s)  *  SLOTS_PER_EPOCH <= SLOTS_PER_HISTORICAL_ROOT 
+        requires get_block_root(s, get_current_epoch(s)) in store.blocks.Keys
+        requires isClosedUnderParent(store)
+
+        /** All the attestations in the state are valid.  */
+        requires forall a :: a in get_matching_target_attestations(s, get_current_epoch(s)) ==>    
+            a.data.beacon_block_root in store.blocks.Keys && isValidAttestation(a.data, store, store.attestations)       
+    
+        ensures 
+            forall a :: a in get_matching_target_attestations(s, get_current_epoch(s)) ==>
+            a.data.source == lastJustifiedCheckPoint(s, store)
+    {
+        
+        forall (a : PendingAttestation | a in get_matching_target_attestations(s, get_current_epoch(s)) )
+            ensures a.data.source == lastJustifiedCheckPoint(s, store)
+        {
+            // assume(isValidAttestation(a.data, store, store.attestations));
+            // //  The chain from a.beacon_block_root
+            // var xc := chainRoots(a.data.beacon_block_root, store);
+            // //  ep(a)
+            // var ep :=  compute_epoch_at_slot(a.data.slot);
+            // //  LEBB(a), LE(a) in the attestation
+            // var indexOfLEBB := computeEBB(xc, ep, store);
+            // //  EBBS
+            // var ebbs := computeAllEBBsIndices(xc, ep, store);
+            // //  Index of Last justified checkpoint in ebbs, LJ(a). in [0..ep]
+            // var indexOfLJ := lastJustified(xc, ebbs, store.attestations) as Epoch;
+            // // assert(a.data.target);
+
+            // assert(a.data.source ==  CheckPoint(ep - indexOfLJ, xc[ebbs[indexOfLJ]]));
+            // assert(|ebbs| == ep as nat + 1);
+            // assert(lastJustifiedCheckPoint(s, store).epoch == |ebbs| as Epoch - 1 - indexOfLJ);
+            // CheckPoint((|ebbs| as Epoch - indexOfLJ) as Epoch, xc[ebbs[indexOfLJ]]));
+
+            assume(a.data.source == lastJustifiedCheckPoint(s, store));
+        }
+    }
+
+
+    /**
+     *  Attestations for current epoch have source the current justified checkpoint.
+     *  @note   ASSUMED
+     */
+    lemma attestationsCurrentEpoch(s : BeaconState, store:  Store)
+        requires s.slot % SLOTS_PER_EPOCH != 0
+        requires get_current_epoch(s) as nat *  SLOTS_PER_EPOCH as nat  <  0x10000000000000000 
+        requires get_current_epoch(s) > GENESIS_EPOCH + 1
+        requires get_current_epoch(s) *  SLOTS_PER_EPOCH   < s.slot  
+        requires s.slot  - get_current_epoch(s)  *  SLOTS_PER_EPOCH <= SLOTS_PER_HISTORICAL_ROOT 
+        requires get_block_root(s, get_current_epoch(s)) in store.blocks.Keys
+        requires isClosedUnderParent(store)
+
+        /** All the attestations in the state are valid.  */
+        requires forall a :: a in get_matching_target_attestations(s, get_current_epoch(s)) ==>    
+            a.data.beacon_block_root in store.blocks.Keys && isValidAttestation(a.data, store, store.attestations)       
+    
+        ensures 
+            forall a :: a in get_matching_target_attestations(s, get_current_epoch(s)) ==>
+            a.data.source == lastJustifiedCheckPoint(s, store)
+    {
+        
+        forall (a : PendingAttestation | a in get_matching_target_attestations(s, get_current_epoch(s)) )
+            ensures a.data.source == lastJustifiedCheckPoint(s, store)
+        {
+            // assume(isValidAttestation(a.data, store, store.attestations));
+            // //  The chain from a.beacon_block_root
+            // var xc := chainRoots(a.data.beacon_block_root, store);
+            // //  ep(a)
+            // var ep :=  compute_epoch_at_slot(a.data.slot);
+            // //  LEBB(a), LE(a) in the attestation
+            // var indexOfLEBB := computeEBB(xc, ep, store);
+            // //  EBBS
+            // var ebbs := computeAllEBBsIndices(xc, ep, store);
+            // //  Index of Last justified checkpoint in ebbs, LJ(a). in [0..ep]
+            // var indexOfLJ := lastJustified(xc, ebbs, store.attestations) as Epoch;
+            // // assert(a.data.target);
+
+            // assert(a.data.source ==  CheckPoint(ep - indexOfLJ, xc[ebbs[indexOfLJ]]));
+            // assert(|ebbs| == ep as nat + 1);
+            // assert(lastJustifiedCheckPoint(s, store).epoch == |ebbs| as Epoch - 1 - indexOfLJ);
+            // CheckPoint((|ebbs| as Epoch - indexOfLJ) as Epoch, xc[ebbs[indexOfLJ]]));
+
+            assume(a.data.source == lastJustifiedCheckPoint(s, store));
+        }
+    }
+
+    /**
+     *  Attestations for previous epoch have source the previous justified checkpoint.
+     *  @note   ASSUMED
+     */
+    lemma attestationsPrevEpoch(s : BeaconState, store:  Store)
+        requires s.slot % SLOTS_PER_EPOCH != 0
+        requires get_current_epoch(s) as nat *  SLOTS_PER_EPOCH as nat  <  0x10000000000000000 
+        requires get_current_epoch(s) > GENESIS_EPOCH + 1
+        requires get_current_epoch(s) *  SLOTS_PER_EPOCH   < s.slot  
+        requires s.slot  - get_current_epoch(s)  *  SLOTS_PER_EPOCH <= SLOTS_PER_HISTORICAL_ROOT 
+        requires get_block_root(s, get_previous_epoch(s)) in store.blocks.Keys
+        requires isClosedUnderParent(store)
+
+        /** All the attestations in the state are valid.  */
+        requires forall a :: a in get_matching_target_attestations(s, get_previous_epoch(s)) ==>    
+            a.data.beacon_block_root in store.blocks.Keys && isValidAttestation(a.data, store, store.attestations)       
+    
+        ensures 
+            forall a :: a in get_matching_target_attestations(s, get_previous_epoch(s)) ==>
+            a.data.source == s.previous_justified_checkpoint
+            && a.data.target == CheckPoint(get_previous_epoch(s),
+                                        get_block_root(s, get_previous_epoch(s)))
+    {
+        
+        forall (a : PendingAttestation | a in get_matching_target_attestations(s, get_previous_epoch(s)) )
+            ensures a.data.source == s.previous_justified_checkpoint 
+            && a.data.target == CheckPoint(get_previous_epoch(s),
+                                        get_block_root(s, get_previous_epoch(s)))
+        {
+    
+            assume(a.data.source == s.previous_justified_checkpoint
+                && a.data.target == CheckPoint(get_previous_epoch(s),
+                                        get_block_root(s, get_previous_epoch(s)))
+                                        );
+        }
+    }
+
+    //  matching target attestations for previous are from previous justified cp
+    //  matching target attestations for current epoch are from last justified.
+
+    //  invariant in the state:
+    //  s.current_epoch_attestations are from s.current_justified_cp (LJ, epoch) to LEBB(epoch)
+    //  s.previous_epoch_attestations are from s.previous_justfified_cp (LJ epoch - 1) to LEBB(epoch  - 1)
+
+    /**
+     *  The checkpoints' status after the process_justification are
+     *  correctly set.
+     */
+    lemma updateJustificationIsCorrect(s : BeaconState, store:  Store) 
+        requires s.slot % SLOTS_PER_EPOCH != 0
+        requires get_current_epoch(s) as nat *  SLOTS_PER_EPOCH as nat  <  0x10000000000000000 
+        requires get_current_epoch(s) > GENESIS_EPOCH + 1
+        requires get_current_epoch(s) *  SLOTS_PER_EPOCH   < s.slot  
+        requires s.slot  - get_current_epoch(s)  *  SLOTS_PER_EPOCH <= SLOTS_PER_HISTORICAL_ROOT 
+        requires get_block_root(s, get_current_epoch(s)) in store.blocks.Keys
+        requires isClosedUnderParent(store)
+        requires isMostRecentJustifiedCheckPoint(s.current_justified_checkpoint, s, store)
+
+        requires isJustifiedCheckPoint(s.previous_justified_checkpoint, s, store)
+        requires isJustifiedCheckPoint(s.current_justified_checkpoint, s, store)
+
+        /** New previous checkpoint in next state is justified. P1 */
+        ensures var s' := updateJustification(s);
+            isJustifiedCheckPoint(s'.previous_justified_checkpoint, s', store)
+        /**  New current checkpoint in next state is justified. P2 */
+        ensures var s' := updateJustificationPrevEpoch(s);
+            isJustifiedCheckPoint(s'.current_justified_checkpoint, s', store)
+    {
+        var s':= updateJustification(s);
+        //  P1 follows from definition 
+        assert(s'.previous_justified_checkpoint == s.current_justified_checkpoint);
+
+        //  Proof of second ensures
+        var s'' :=  updateJustificationPrevEpoch(s);
+        //  get attestations in state for previous epoch.
+        var matching_target_attestations_prev_epoch := 
+                get_matching_target_attestations(s, get_previous_epoch(s));
+        var b1 := get_attesting_balance(s, matching_target_attestations_prev_epoch) as nat * 3 
+                        >= get_total_active_balance(s) as nat * 2;
+        if b1 {
+            //  there is a supermajority for the checkpoint at previous epoch.
+            //  because of the constraints on attestations in the state, this must
+            //  be from the prev_justified_checkpoint which is justified.
+            //  Proof that supermajority in 
+            //  get_matching_target_attestations(s, get_previous_epoch(s)) must have 
+            //  source s.current_justified_checkpoint
+            assert(isJustifiedCheckPoint(s.previous_justified_checkpoint, s, store));
+            // assert( isJustifiedCheckPoint());
+            //  Hence this checkpoint is justified
+            assume( isJustifiedCheckPoint(s''.current_justified_checkpoint, s', store));
+        } else {
+            assert(s''.current_justified_checkpoint ==  s.current_justified_checkpoint);
+        }
+        
+    }
+
+    lemma justificationFromPreviousAndSuper(s : BeaconState, store:  Store) 
+        requires s.slot % SLOTS_PER_EPOCH != 0
+        requires get_current_epoch(s) as nat *  SLOTS_PER_EPOCH as nat  <  0x10000000000000000 
+        requires get_current_epoch(s) > GENESIS_EPOCH + 1
+        requires get_current_epoch(s) *  SLOTS_PER_EPOCH   < s.slot  
+        requires s.slot  - get_current_epoch(s)  *  SLOTS_PER_EPOCH <= SLOTS_PER_HISTORICAL_ROOT 
+        requires get_block_root(s, get_current_epoch(s)) in store.blocks.Keys
+        requires get_block_root(s, get_previous_epoch(s)) in store.blocks.Keys
+
+        requires isClosedUnderParent(store)
+        requires isMostRecentJustifiedCheckPoint(s.current_justified_checkpoint, s, store)
+
+        requires isJustifiedCheckPoint(s.previous_justified_checkpoint, s, store)
+        requires isJustifiedCheckPoint(s.current_justified_checkpoint, s, store)
+
+        /** All the attestations in the state are valid.  */
+        requires forall a :: a in get_matching_target_attestations(s, get_previous_epoch(s)) ==>    
+            a.data.beacon_block_root in store.blocks.Keys && isValidAttestation(a.data, store, store.attestations)   
+
+        requires 
+            var matching_target_attestations_prev_epoch := 
+                get_matching_target_attestations(s, get_previous_epoch(s));
+            get_attesting_balance(s, matching_target_attestations_prev_epoch) as nat * 3 
+                        >= get_total_active_balance(s) as nat * 2
+        
+        // ensures 
+        //     var previous_epoch := get_previous_epoch(s);
+        //     isJustifiedCheckPoint(CheckPoint(previous_epoch,
+        //                                 get_block_root(s, previous_epoch)), s, store)
+    {
+        var r := get_block_root(s, get_current_epoch(s));
+        var roots := chainRoots(r, store); 
+        var ebbsIndices := computeAllEBBsIndices(roots, get_current_epoch(s), store);
+        assert(exists i :: 0 <= i < |ebbsIndices| && isJustified(i, roots, ebbsIndices, store.attestations)
+            && s.previous_justified_checkpoint == CheckPoint((|ebbsIndices| - i) as Epoch, roots[ebbsIndices[i]]));
+        
+        //  1. attestations in prev_epoch are from s.previous_justified_checkpoint  to 
+        //  CheckPoint(previous_epoch, get_block_root(s, previous_epoch))
+        //  2. apply inductive def of isJustified
+        attestationsPrevEpoch(s, store);
+        //  attestations are from s.previous_justified_checkpoint to LEBB(prev_epoch)
+        assert(forall a :: a in get_matching_target_attestations(s, get_previous_epoch(s)) ==>
+            a.data.source == s.previous_justified_checkpoint
+            && a.data.target == CheckPoint(get_previous_epoch(s),
+                                        get_block_root(s, get_previous_epoch(s))));
+        //  because s.previous_justified_checkpoint is justified and supermajority to 
+        //  cp == CheckPoint(get_previous_epoch(s),get_block_root(s, get_previous_epoch(s))))
+        //  it follows that cp is justified.
+    }
+  
+}
